Refactoring: using dummy locales to simplify formulas

PDDL_Normalization.thy
@@ -50,8 +50,7 @@ locale restr_problem = wf_ast_problem +
 begin
   sublocale restr_domain "domain P"
     apply unfold_locales
-    using restrP
-    unfolding restrict_prob_def by simp
+    using restrP restrict_prob_def by simp
 
   lemma single_t_cnsts: "singleton_types (objects P)"
     using restrP by (auto simp add: restrict_dom_def restrict_prob_def)
@@ -176,179 +175,134 @@ definition (in ast_problem) normalized_prob :: "bool" where
 
 (* ------------------------------------- PROOFS ------------------------------------------------- *)
 
-text \<open>This is mostly to simplify the syntax, actually. So I can just do
-   \<open>Dt.some_function\<close> instead of \<open>ast_domain.some_function detype_dom\<close>.
-    But I'm not using it (yet) as the cleaner syntax doesn't offset the added confusion.\<close>
-(*locale ast_domain2 = ast_domain
-sublocale ast_domain2 \<subseteq> Dt: ast_domain detype_dom .
-locale wf_ast_domain2 = wf_ast_domain
-sublocale wf_ast_domain2 \<subseteq> Dt: ast_domain detype_dom .
-locale ast_problem2 = ast_problem
-sublocale ast_problem2 \<subseteq> Pt: ast_problem detype_prob . *)
-
 subsection \<open>Type Normalization Proofs\<close>
 
-subsubsection \<open> Type Normalization Produces Typeless PDDL \<close>
+text \<open>This is only to simplify the syntax. So I can just do
+   \<open>d2.some_function\<close> instead of \<open>ast_domain.some_function detype_dom\<close>.\<close>
+abbreviation (in ast_domain) (input) "D2 \<equiv> detype_dom"
+abbreviation (in ast_problem) (input) "P2 \<equiv> detype_prob"
+
+locale ast_domain2 = ast_domain
+sublocale ast_domain2 \<subseteq> d2: ast_domain D2 .
+
+locale wf_ast_domain2 = wf_ast_domain
+sublocale wf_ast_domain2 \<subseteq> d2: ast_domain D2 .
+sublocale wf_ast_domain2 \<subseteq> ast_domain2 .
+
+locale restr_domain2 = restr_domain
+sublocale restr_domain2 \<subseteq> d2 : ast_domain D2 .
+sublocale restr_domain2 \<subseteq> wf_ast_domain2
+  apply unfold_locales .
+
+locale ast_problem2 = ast_problem
+sublocale ast_problem2 \<subseteq> p2: ast_problem P2 .
+sublocale ast_problem2 \<subseteq> ast_domain2 D .
+
+locale wf_ast_problem2 = wf_ast_problem
+sublocale wf_ast_problem2 \<subseteq> p2 : ast_problem P2.
+sublocale wf_ast_problem2 \<subseteq> ast_problem2 .
+sublocale wf_ast_problem2 \<subseteq> wf_ast_domain2 D
+  apply unfold_locales .
+
+locale restr_problem2 = restr_problem
+sublocale restr_problem2 \<subseteq> p2 : ast_problem P2 .
+sublocale restr_problem2 \<subseteq> wf_ast_problem2
+  apply unfold_locales .
+sublocale restr_problem2 \<subseteq> restr_domain2 D
+  apply unfold_locales .
 
 context ast_domain
 begin
 
-  lemma preds_detyped: "\<forall>p \<in> set (predicates detype_dom). \<forall>T \<in> set (argTs p). T = \<omega>"
-    using type_preds_def detype_preds_def detype_dom_def by auto
+text \<open> basic stuff \<close>
+
+  lemma (in -) dist_pred: "distinct names \<longleftrightarrow> distinct (map Pred names)"
+    by (meson distinct_map inj_onI predicate.inject)
+
+  lemmas (in wf_ast_domain) wf_dom_def = wf_domain[unfolded wf_domain_def]
   
-  lemma ents_detyped: "\<forall>(n, T) \<in> set (detype_ents ents). T = \<omega>"
-    unfolding detype_ents_def
-    by (simp add: case_prod_beta' detype_dom_def)
+  lemmas (in wf_ast_problem) wf_prob_def = wf_problem[unfolded wf_problem_def]
 
+text \<open> type system \<close>
 
+  lemma (in -) wf_object: "ast_domain.wf_type d \<omega>"
+    unfolding ast_domain.wf_type.simps by simp
 
-  lemma ac_params_detyped:
-    "\<forall>ac \<in> set (actions detype_dom). \<forall>(n, T) \<in> set (parameters ac). T = \<omega>"
-    using detype_dom_def detype_ac_def ents_detyped by fastforce
-  
-  lemma dom_detyped:
-    "ast_domain.typeless_dom detype_dom"
-  proof -
-    have c1: "types detype_dom = []" using detype_dom_def by simp
-    note c2 = preds_detyped
-    have c3: "\<forall>(n, T) \<in> set (consts detype_dom). T = \<omega>"
-      by (simp add: detype_dom_def ents_detyped)
-    note c4 = ac_params_detyped
-  
-    from c1 c2 c3 c4 show ?thesis
-      using ast_domain.typeless_dom_def by simp
-  qed
-end
-
-lemma (in ast_problem) prob_detyped:
-  "ast_problem.typeless_prob detype_prob"
-proof -
-  have "\<forall>(n, T) \<in> set (objects detype_prob). T = \<omega>"
-    by (simp add: detype_prob_def ents_detyped)
-  thus ?thesis using dom_detyped ast_problem.typeless_prob_def detype_prob_def by simp
-qed
-
-subsubsection \<open> Type Normalization Preserves Well-Formedness \<close>
-
-(* Properties of type system *)
-
-context ast_domain
-begin
-  
-  lemma subtype_edge_swap: "subtype_edge = prod.swap"
+  lemma subtype_edge_swap:
+    "subtype_edge = prod.swap"
   proof -
     have "\<And>a b. subtype_edge (a, b) = prod.swap (a, b)"
       by simp
     thus ?thesis by fast
   qed
-  
-  lemma wf_object: "ast_domain.wf_type d \<omega>"
-    unfolding ast_domain.wf_type.simps by simp
 
   lemma tyterm_prop: "P (ty_term varT cnstT x) \<longleftrightarrow>
     (case x of term.VAR x' \<Rightarrow> P (varT x') |
                term.CONST x' \<Rightarrow> P (cnstT x'))"
     apply (split term.split)
     by simp
-  
+
   lemma tyterm_elem: "(ty_term (map_of varT) (map_of cnstT) x \<noteq> None)
     \<longleftrightarrow> (case x of term.VAR x' \<Rightarrow> x' \<in> fst ` set varT |
                    term.CONST x' \<Rightarrow> x' \<in> fst ` set cnstT)"
     apply (split term.split)
     using tyterm_prop by (simp add: map_of_eq_None_iff)
 
-  (* supertype enumeration *)
-  
-  lemma wf_type_iff_listed: "wf_type (Either ts) \<longleftrightarrow> (\<forall>t \<in> set ts. t \<in> set (type_names))"
+text \<open> type_names \<close>
+
+ lemma wf_type_iff_listed: "wf_type T \<longleftrightarrow> (\<forall>t \<in> set (primitives T). t \<in> set (type_names))"
   proof -
     have "set type_names = insert ''object'' (fst ` set (types D))"  by auto
-    thus ?thesis by (simp add: subset_code(1))
+    hence "wf_type (Either ts) \<longleftrightarrow> (\<forall>t \<in> set ts. t \<in> set (type_names))" for ts
+      by (simp add: subset_code(1))
+    thus ?thesis using type.collapse by metis
   qed
 
-  lemma of_type_iff_reach:
-    shows "of_type oT T \<longleftrightarrow> (
-      \<forall>ot \<in> set (primitives oT).
-      \<exists>t \<in> set (primitives T).
-        t \<in> set (supertypes_of ot))"
-  proof -
-    have "subtype_rel = set (map prod.swap (types D))"
-      using subtype_rel_def subtype_edge_swap by metis
-    hence subrel_inv: "subtype_rel = (set (types D))\<inverse>" by auto
-    hence "of_type oT T \<longleftrightarrow>
-      set (primitives oT) \<subseteq> ((set (types D))\<inverse>)\<^sup>* `` set (primitives T)"
-      using of_type_def by simp
-    also have "... \<longleftrightarrow>
-      set (primitives oT) \<subseteq> ((set (types D))\<^sup>*)\<inverse> `` set (primitives T)"
-      by (simp add: rtrancl_converse)
-    also have "... \<longleftrightarrow>
-      (\<forall>ot \<in> set (primitives oT). ot \<in> ((set (types D))\<^sup>*)\<inverse> `` set (primitives T))"
-      by auto
-    also have "... \<longleftrightarrow>
-      (\<forall>ot \<in> set (primitives oT). \<exists>t. (ot, t) \<in> (set (types D))\<^sup>* \<and> t \<in> set (primitives T))"
-      by auto
-    finally show ?thesis using reachable_iff_in_star by metis
-  qed
+text \<open> pred_for_type \<close>
 
   lemma type_preds_ids: "map pred type_preds = map pred_for_type type_names"
     using type_preds_def by simp
 
-  lemma p_is_tp: "p \<in> pred ` set type_preds \<longleftrightarrow> (\<exists>t \<in> set type_names. p = pred_for_type t)"
-  (* by force takes 9 seconds *)
+  lemma type_pred_refs_type: "p \<in> pred ` set type_preds \<longleftrightarrow> (\<exists>t \<in> set type_names. p = pred_for_type t)"
   proof -
     have "pred ` set type_preds = pred_for_type ` set type_names"
       by (metis type_preds_ids list.set_map)
     thus ?thesis by auto
   qed
-end
 
+text \<open> type_preds \<close>
 
-lemma (in ast_problem) obj_of_type_iff_reach:
-  assumes "objT n = Some oT"
-  shows  "is_obj_of_type n T \<longleftrightarrow>
-    (\<forall>ot \<in> set (primitives oT).
-      \<exists>t \<in> set (primitives T).
-    t \<in> set (supertypes_of ot))"
-  using assms is_obj_of_type_def of_type_iff_reach by auto
-
-lemma (in ast_domain) single_of_type_iff:
-  shows "of_type (Either [ot]) T \<longleftrightarrow> (
-    \<exists>t \<in> set (primitives T).
-      t \<in> set (supertypes_of ot))"
-  using of_type_iff_reach by simp
-
-lemma (in ast_problem) simple_obj_of_type_iff:
-  assumes "objT n = Some (Either [ot])"
-  shows  "is_obj_of_type n T \<longleftrightarrow>
-      (\<exists>t \<in> set (primitives T).
-    t \<in> set (supertypes_of ot))"
-  using assms is_obj_of_type_def single_of_type_iff by auto
-
-(* well-formedness *)
-
-lemma dist_pred: "distinct names \<longleftrightarrow> distinct (map Pred names)"
-  by (meson distinct_map inj_onI predicate.inject)
-
-context ast_domain
-begin
-  lemmas (in wf_ast_domain) wf_dom_def = wf_domain[unfolded wf_domain_def]
-
-  lemma dt_pred_name: "pred (detype_pred pd) = pred pd" by simp
-  lemma dt_preds_names:
-    "map pred (detype_preds ps) = map pred ps"
-    using dt_pred_name detype_preds_def by simp
   lemma tps_dis:
     "distinct (map pred type_preds)" (is "distinct ?tp_ids")
   proof -
     let ?pred_ids = "map pred (predicates D)"
     let ?prefix = "safe_prefix (map predicate.name ?pred_ids)"
     have tp_ids: "?tp_ids = map (Pred \<circ> ((@) ?prefix)) type_names"
-        by (simp add: type_preds_def)
+        by (simp add: type_preds_ids)
     have "distinct (map ((@) ?prefix) type_names)" (* because: distinct type_names *)
       using dist_prefix by simp
     hence "distinct (map (Pred \<circ> ((@) ?prefix)) type_names)"
       using dist_pred by simp
     thus "distinct ?tp_ids" using tp_ids by metis
   qed
+
+text \<open> supertype preds \<close>
+
+text \<open> supertype facts \<close>
+
+text \<open> type conds/preconds \<close>
+
+text \<open> detyped preds \<close>
+
+  lemma preds_detyped:
+    "\<forall>p \<in> set (predicates D2). \<forall>T \<in> set (argTs p). T = \<omega>"
+    using type_preds_def detype_preds_def detype_dom_def by auto
+
+  lemma dt_pred_name: "pred (detype_pred pd) = pred pd" by simp
+
+  lemma dt_preds_names:
+    "map pred (detype_preds ps) = map pred ps"
+    using dt_pred_name detype_preds_def by simp
 
   (* TODO simplify *)
   lemma tps_dt_preds_disj:
@@ -381,7 +335,7 @@ begin
   qed
 
   lemma (in wf_ast_domain) t_preds_dis:
-    shows "distinct (map pred (predicates detype_dom))"
+    shows "distinct (map pred (predicates D2))"
   proof -
     (* Predicate names are unique because the original predicate names are unchanged
        and the additional predicate names are unique (based on unique type names)
@@ -396,16 +350,21 @@ begin
     thus ?thesis using ast_domain.sel(2) detype_dom_def by presburger
   qed
 
-  lemma t_preds_wf:
-      "\<forall>p \<in> set (predicates detype_dom). ast_domain.wf_predicate_decl detype_dom p"
-    proof -
-      have "\<forall>p \<in> set (predicates detype_dom). \<forall>T \<in> set (argTs p). T = \<omega>"
-        by (rule preds_detyped)
-      hence "\<forall>p \<in> set (predicates detype_dom). \<forall>T \<in> set (argTs p). ast_domain.wf_type detype_dom T"
-        using preds_detyped wf_object by auto
-      thus ?thesis by (metis ast_domain.wf_predicate_decl.simps predicate_decl.collapse)
-    qed
-  
+  lemma (in ast_domain2) t_preds_wf:
+    "\<forall>p \<in> set (predicates D2). d2.wf_predicate_decl p"
+  proof -
+    have "\<forall>p \<in> set (predicates D2). \<forall>T \<in> set (argTs p). T = \<omega>"
+      by (rule preds_detyped)
+    hence "\<forall>p \<in> set (predicates D2). \<forall>T \<in> set (argTs p). d2.wf_type T"
+      using preds_detyped wf_object by auto
+    thus ?thesis by (metis d2.wf_predicate_decl.simps predicate_decl.collapse)
+  qed
+
+text \<open> detype ents \<close>
+
+  lemma ents_detyped: "\<forall>(n, T) \<in> set (detype_ents ents). T = \<omega>"
+    by (simp add: detype_ents_def case_prod_beta' detype_dom_def)
+
   lemma t_ents_names:
     "map fst (detype_ents ents) = map fst ents"
     unfolding detype_ents_def by auto
@@ -415,11 +374,29 @@ begin
     shows "distinct (map fst (detype_ents ents))"
     using assms by (metis t_ents_names)
 
-  lemma t_ents_wf:
-    shows "(\<forall>(n,T)\<in>set (detype_ents ents). ast_domain.wf_type detype_dom T)"
+  lemma (in ast_domain2) t_ents_wf:
+    shows "(\<forall>(n,T) \<in> set (detype_ents ents). d2.wf_type T)"
     using ents_detyped wf_object by fast
 
-  (* predicate signatures *)
+(* stuff for formulas later *)
+
+  lemma t_entT_Some:
+    shows "map_of ents x \<noteq> None \<longleftrightarrow> map_of (detype_ents ents) x = Some \<omega>"
+  proof -
+    have 1: "\<forall>T \<in> snd ` set (detype_ents ents). T = \<omega>" using ents_detyped by fastforce
+    have "map_of ents x \<noteq> None \<longleftrightarrow> x \<in> fst ` set ents" using map_of_eq_None_iff by metis
+    also have "... \<longleftrightarrow> x \<in> fst ` set (detype_ents ents)" using t_ents_names by (metis list.set_map)
+    
+    ultimately show ?thesis using 1 map_of_in_R_iff
+      by (metis map_of_eq_None_iff option.discI)
+  qed
+
+  lemma t_entT_None:
+    shows "map_of ents x = None \<longleftrightarrow> map_of (detype_ents ents) x = None"
+    using t_ents_names list.set_map map_of_eq_None_iff by metis
+
+text \<open> predicate signatures \<open>sig\<close> \<close>
+
   abbreviation "split_pred \<equiv> (\<lambda>PredDecl p n \<Rightarrow> (p, n))"
 
   lemma pred_resolve:
@@ -450,12 +427,11 @@ begin
 
   text \<open>Decompose the signature function of the detyped domain in two ways, since the domains
     are disjoint. Yes this is the best way I could think of.\<close>
-  lemma t_sig_split_a:
-    "ast_domain.sig detype_dom =
+  lemma (in ast_domain2) t_sig_split_a:
+    "d2.sig =
       map_of (map split_pred (detype_preds (predicates D))) ++ map_of (map split_pred type_preds)"
   proof -
-    interpret d2 : ast_domain detype_dom .
-    let ?pred_map2 = "(map split_pred (predicates detype_dom))"
+    let ?pred_map2 = "(map split_pred (predicates D2))"
     let ?t_pred_map = "map split_pred type_preds"
     let ?dt_pred_map = "map split_pred (detype_preds (predicates D))"
 
@@ -471,14 +447,13 @@ begin
   qed
 
   (* d2.sig maps interchangable *)
-  lemma (in wf_ast_domain) t_sig_split_b:
-    "ast_domain.sig detype_dom =
+  lemma (in wf_ast_domain2) t_sig_split_b:
+    "d2.sig =
       map_of (map split_pred type_preds) ++ map_of (map split_pred (detype_preds (predicates D)))"
   proof -
-    interpret d2 : ast_domain detype_dom .
     have dis: "distinct (map pred (predicates D))" using wf_dom_def by simp
 
-    let ?pred_map2 = "(map split_pred (predicates detype_dom))"
+    let ?pred_map2 = "(map split_pred (predicates D2))"
     let ?t_pred_map = "map split_pred type_preds"
     let ?dt_pred_map = "map split_pred (detype_preds (predicates D))"
 
@@ -495,15 +470,14 @@ begin
     thus ?thesis using t_sig_split_a by simp
   qed
 
-  lemma (in wf_ast_domain) t_sig_some:
-    "ast_domain.sig detype_dom p \<noteq> None \<longleftrightarrow>
+  lemma (in wf_ast_domain2) t_sig_some:
+    "d2.sig p \<noteq> None \<longleftrightarrow>
       (p \<in> pred ` set (predicates D))
       \<or> (p \<in> pred_for_type ` set type_names)"
   proof -
-    interpret d2 : ast_domain detype_dom .
     have dis: "distinct (map pred (predicates D))" using wf_dom_def by simp
 
-    let ?pred_map2 = "(map split_pred (predicates detype_dom))"
+    let ?pred_map2 = "(map split_pred (predicates D2))"
     let ?t_pred_map = "map split_pred type_preds"
     let ?dt_pred_map = "map split_pred (detype_preds (predicates D))"
 
@@ -528,9 +502,9 @@ begin
 
   (* Using distinctness of predicates is a shortcut here.
      It's technically not required because the order of predicates is unchanged.*)
-  lemma (in wf_ast_domain) t_preds_arity:
+  lemma (in wf_ast_domain2) t_preds_arity:
     assumes "sig p = Some Ts"
-    shows "ast_domain.sig detype_dom p = Some (replicate (length Ts) \<omega>)"
+    shows "d2.sig p = Some (replicate (length Ts) \<omega>)"
   proof -
     have dis: "distinct (map pred (predicates D))" using wf_dom_def by simp
     let ?dt_pred_map = "map split_pred (detype_preds (predicates D))"
@@ -543,95 +517,67 @@ begin
     thus ?thesis using t_sig_split_b by simp
   qed
 
-  lemma "map_of m x \<noteq> None \<longleftrightarrow> x \<in> fst ` set m"
-    by (simp add: map_of_eq_None_iff)
 
-  (* formulas *)
+text \<open> type maps \<close>
 
-  lemma "constT x \<noteq> None \<longleftrightarrow> (x \<in> fst ` set (consts D))"
-    using constT_def by (simp add: map_of_eq_None_iff)
+  lemma (in ast_domain2) t_constT_Some: "constT c \<noteq> None \<longleftrightarrow> d2.constT c = Some \<omega>"
+    using t_entT_Some ast_domain.constT_def detype_dom_def by fastforce
 
-  lemma t_entT:
-    assumes "x \<in> fst ` set ents"
-    shows "map_of (detype_ents ents) x = Some \<omega>"
+  lemma (in ast_domain2) t_constT_None: "constT c = None \<longleftrightarrow> d2.constT c = None"
+    using t_entT_None ast_domain.constT_def detype_dom_def by fastforce
+
+  lemma (in ast_problem2) t_objT_Some: "objT c \<noteq> None \<longleftrightarrow> p2.objT c = Some \<omega>"
   proof -
-    have "map fst ents = map fst (detype_ents ents)" using t_ents_names by metis
-    hence x: "x \<in> fst ` set (detype_ents ents)" using assms by (metis image_set)
-    have "\<forall>T \<in> snd ` set (detype_ents ents). T = \<omega>"
-      using ents_detyped by fastforce
-    thus ?thesis
-      using x img_snd map_of_SomeD map_of_eq_None_iff option.exhaust by metis
-  qed
-
-  lemma "\<forall>y \<in> snd ` set m. y = r \<Longrightarrow> x \<in> fst ` set m \<Longrightarrow> map_of m x = Some r"
-    by (metis img_snd in_fst_imageE map_of_SomeD weak_map_of_SomeI)
-
-  lemma "snd ` set m = {r} \<Longrightarrow> x \<in> fst ` set m \<Longrightarrow> map_of m x = Some r"
-    by (metis emptyE img_snd in_fst_imageE insertE map_of_SomeD weak_map_of_SomeI)
-
-  lemma t_entT_alt:
-    shows "map_of ents x \<noteq> None \<longleftrightarrow> map_of (detype_ents ents) x = Some \<omega>"
-  proof -
-    have 1: "\<forall>T \<in> snd ` set (detype_ents ents). T = \<omega>" using ents_detyped by fastforce
-    have "map_of ents x \<noteq> None \<longleftrightarrow> x \<in> fst ` set ents" using map_of_eq_None_iff by metis
-    also have "... \<longleftrightarrow> x \<in> fst ` set (detype_ents ents)" using t_ents_names by (metis list.set_map)
-    ultimately show ?thesis using 1
-      by (metis map_of_eq_None_iff option.distinct(1) t_entT)
-  qed
-
-  lemma t_entT_None:
-    shows "map_of ents x = None \<longleftrightarrow> map_of (detype_ents ents) x = None" sorry
-
-  lemma t_constT: "constT c \<noteq> None \<longleftrightarrow> ast_domain.constT detype_dom c = Some \<omega>"
-    using t_entT_alt ast_domain.constT_def detype_dom_def by fastforce
-
-  lemma "m1 x = Some y \<or> m1 x = None \<and> m2 x = Some y \<Longrightarrow> (m2 ++ m1) x = Some y"
-    by (simp add: map_add_Some_iff)
-
-  lemma (in ast_problem) t_objT: "objT c \<noteq> None \<longleftrightarrow> ast_problem.objT detype_prob c = Some \<omega>"
-  proof -
-    interpret p2 : ast_problem detype_prob .
-    have o1: "objT = map_of (objects P) ++ constT" using objT_def by simp
-
-    have "objT c \<noteq> None \<longleftrightarrow> constT c \<noteq> None \<or> constT c = None \<and> map_of (objects P) c \<noteq> None" using objT_def by auto
-    also have "... \<longleftrightarrow> p2.constT c = Some \<omega> \<or> p2.constT c = None \<and> map_of (objects P) c \<noteq> None"
-      using t_constT t_entT_None detype_prob_def sorry
+    have "objT c \<noteq> None \<longleftrightarrow> constT c \<noteq> None \<or> constT c = None \<and> map_of (objects P) c \<noteq> None"
+      using objT_def by auto
+    also have "... \<longleftrightarrow> constT c \<noteq> None \<or> constT c = None \<and> map_of (objects detype_prob) c = Some \<omega>"
+      using detype_prob_def t_entT_Some by fastforce
+    also have "... \<longleftrightarrow> p2.constT c = Some \<omega> \<or> constT c = None \<and> map_of (objects detype_prob) c = Some \<omega>"
+      using detype_prob_def t_constT_Some by fastforce
     also have "... \<longleftrightarrow> p2.constT c = Some \<omega> \<or> p2.constT c = None \<and> map_of (objects detype_prob) c = Some \<omega>"
-      using t_entT_alt detype_prob_def by fastforce
-    also have "... \<longleftrightarrow> p2.constT c = Some \<omega> \<or> p2.constT c = None \<and> map_of (objects detype_prob) c = Some \<omega>"
-      using t_entT_None detype_prob_def by fastforce
-    also have "... \<longleftrightarrow> (map_of (objects detype_prob) ++ p2.constT) c = Some \<omega>" using map_add_Some_iff sorry
-    (* also have "... \<longleftrightarrow> p2.objT c = Some \<omega>" sorry *)
-
-    ultimately show ?thesis sorry
+      using detype_prob_def t_constT_None by fastforce
+    also have "... \<longleftrightarrow> (map_of (objects detype_prob) ++ p2.constT) c = Some \<omega>"
+      using map_add_Some_iff by fastforce
+    also have "... \<longleftrightarrow> p2.objT c = Some \<omega>" using p2.objT_def by simp
+    ultimately show ?thesis by simp
   qed
 
+  lemma (in ast_problem2) t_objT_None: "objT c = None \<longleftrightarrow> p2.objT c = None"
+    using t_entT_None ast_problem.objT_def
+    by (metis ast_problem.sel(1-2) detype_prob_def map_add_None t_constT_None)
 
-  lemma t_cnstT_some:
+   lemma t_tyt_const_Some:
     assumes "ty_term vT (map_of cnsts) (term.CONST x) \<noteq> None"
     shows "ty_term vT' (map_of (detype_ents cnsts)) (term.CONST x) = Some \<omega>"
-    using assms t_entT by (metis map_of_eq_None_iff ty_term.simps(2))
+    using assms t_entT_Some by (metis ty_term.simps(2))
 
-  lemma t_varT_some:
+  lemma t_tyt_var_Some:
     assumes "ty_term (map_of vars) cT (term.VAR x) \<noteq> None"
     shows "ty_term (map_of (detype_ents vars)) cT' (term.VAR x) = Some \<omega>"
-    using assms t_entT by (metis map_of_eq_None_iff ty_term.simps(1))
+    using assms t_entT_Some by (metis ty_term.simps(1))
 
-  lemma t_tyt_some:
+  lemma t_tyt_Some:
     assumes "ty_term (map_of vars) (map_of cnsts) e \<noteq> None"
     shows "ty_term (map_of (detype_ents vars)) (map_of (detype_ents cnsts)) e = Some \<omega>"
     using assms apply (induction e)
-    apply (metis t_entT map_of_eq_None_iff ty_term.simps(1))
-    apply (metis t_entT map_of_eq_None_iff ty_term.simps(2))
+    apply (metis t_entT_Some ty_term.simps(1))
+    apply (metis t_entT_Some ty_term.simps(2))
     done
 
-  thm of_type_refl
-  lemma t_tyt_params:
+  lemma t_tyt_None:
+    assumes "ty_term (map_of vars) (map_of cnsts) e = None"
+    shows "ty_term (map_of (detype_ents vars)) (map_of (detype_ents cnsts)) e = None"
+    using assms apply (induction e)
+    apply (metis t_entT_None ty_term.simps(1))
+    apply (metis t_entT_None ty_term.simps(2))
+    done
+
+  (* See \<open>t_ac_tyt\<close> for where the assumption comes from. *)
+  lemma (in ast_domain2) t_tyt_params:
     assumes "\<forall>e. tyt e \<noteq> None \<longrightarrow> tyt2 e = Some \<omega>"
       "list_all2 (is_of_type tyt) params Ts"
-    shows "list_all2 (ast_domain.is_of_type detype_dom tyt2) params (replicate (length Ts) \<omega>)"
+    shows "list_all2 (d2.is_of_type tyt2) params (replicate (length Ts) \<omega>)"
   proof -
-    interpret d2 : ast_domain detype_dom .
     from assms(2) have
       ls: "length params = length Ts" and
       "\<forall>i < length params. is_of_type tyt (params !i) (Ts ! i)"
@@ -648,34 +594,32 @@ begin
       by (simp add: list_all2_conv_all_nth)
   qed
 
+text \<open> formulas \<close>
+
   thm wf_pred_atom.simps
-  lemma (in wf_ast_domain) t_atom_wf:
+  lemma (in wf_ast_domain2) t_atom_wf:
     assumes "\<forall>e. tyt e \<noteq> None \<longrightarrow> tyt2 e = Some \<omega>"
       "wf_atom tyt a"
-    shows "ast_domain.wf_atom detype_dom tyt2 a"
-  proof -
-    interpret d2 : ast_domain detype_dom .
-    from assms show ?thesis
-    proof (induction a)
-      case (predAtm p params)
-      (* these follow from the definition of wf_pred_atom *)
-      then obtain Ts where sigp: "sig p = Some Ts" by fastforce
-      from predAtm this have 1: "list_all2 (is_of_type tyt) params Ts" by simp
+    shows "d2.wf_atom tyt2 a"
+    using assms
+  proof (induction a)
+    case (predAtm p params)
+    (* these follow from the definition of wf_pred_atom *)
+    then obtain Ts where sigp: "sig p = Some Ts" by fastforce
+    from predAtm this have 1: "list_all2 (is_of_type tyt) params Ts" by simp
 
-      let ?os = "replicate (length Ts) \<omega>"
-      from assms 1 have a: "list_all2 (d2.is_of_type tyt2) params ?os"
-        by (simp add: t_tyt_params)
-      have b: "d2.sig p = Some ?os" using sigp by (simp add: t_preds_arity)
+    let ?os = "replicate (length Ts) \<omega>"
+    from assms 1 have a: "list_all2 (d2.is_of_type tyt2) params ?os"
+      by (simp add: t_tyt_params)
+    have b: "d2.sig p = Some ?os" using sigp by (simp add: t_preds_arity)
 
-      from a b show ?case by
-        (simp add: ast_domain.wf_pred_atom.simps ast_domain.wf_atom.simps(1))
-    qed simp
-  qed
+    from a b show ?case by simp
+  qed simp
 
-  lemma (in wf_ast_domain) t_fmla_wf:
+  lemma (in wf_ast_domain2) t_fmla_wf:
     assumes "\<forall>e. tyt e \<noteq> None \<longrightarrow> tyt2 e = Some \<omega>"
       "wf_fmla tyt \<phi>"
-    shows "ast_domain.wf_fmla detype_dom tyt2 \<phi>"
+    shows "d2.wf_fmla tyt2 \<phi>"
     using assms apply (induction \<phi>)
     using t_atom_wf ast_domain.wf_fmla.simps(1) apply blast
     using ast_domain.wf_fmla.simps(2) apply blast
@@ -684,10 +628,10 @@ begin
     using ast_domain.wf_fmla.simps(4) apply blast
     using ast_domain.wf_fmla.simps(6) by metis
 
-  lemma (in wf_ast_domain) t_fmla_atom_wf:
+  lemma (in wf_ast_domain2) t_fmla_atom_wf:
     assumes "\<forall>e. tyt e \<noteq> None \<longrightarrow> tyt2 e = Some \<omega>"
       "wf_fmla_atom tyt \<phi>"
-    shows "ast_domain.wf_fmla_atom detype_dom tyt2 \<phi>"
+    shows "d2.wf_fmla_atom tyt2 \<phi>"
     using assms
     by (simp add: ast_domain.wf_fmla_atom_alt t_fmla_wf)
 
@@ -698,52 +642,13 @@ begin
     using wf_effect.simps ast_effect.collapse
     by metis (* TODO how to just manipulate this lemma with options? *)
 
-  lemma (in wf_ast_domain) t_eff_wf:
+  lemma (in wf_ast_domain2) t_eff_wf:
     assumes "\<forall>e. tyt e \<noteq> None \<longrightarrow> tyt2 e = Some \<omega>"
       "wf_effect tyt \<epsilon>"
-    shows "ast_domain.wf_effect detype_dom tyt2 \<epsilon>"
+    shows "d2.wf_effect tyt2 \<epsilon>"
     using assms ast_domain.wf_effect_alt t_fmla_atom_wf by blast
 
-
-  (* actions *)
-  abbreviation (in ast_domain) "ac_name \<equiv> ast_action_schema.name"
-  (* abbreviation (in ast_domain) "ac_params \<equiv> ast_action_schema.parameters" \<comment> just use \<open>parameters\<close> *)
-  abbreviation (in ast_domain) "ac_pre \<equiv> ast_action_schema.precondition"
-  abbreviation (in ast_domain) "ac_eff \<equiv> ast_action_schema.effect"
-
-  lemma t_ac_name: "ac_name (detype_ac ac) = ac_name ac"
-    by (simp add: detype_ac_def)
-  lemma t_acs_names: "map ac_name (map detype_ac acs) = map ac_name acs"
-    by (simp add: t_ac_name)
-  lemma (in wf_ast_domain) t_acs_dis:
-    "distinct (map ac_name (map detype_ac (actions D)))"
-    using t_acs_names wf_dom_def by metis
-
-  (* TODO just manipulate lemma  *)
-  lemma (in ast_domain) wf_ac_expanded:
-    "wf_action_schema a \<longleftrightarrow> (
-      let
-        tyt = ty_term (map_of (parameters a)) constT
-      in
-        distinct (map fst (parameters a))
-      \<and> wf_fmla tyt (ac_pre a)
-      \<and> wf_effect tyt (ac_eff a))"
-    using wf_action_schema.simps
-    by (metis ast_action_schema.collapse)
-
-  lemma t_ac_tyt:
-    assumes "ty_term (map_of (parameters a)) constT x \<noteq> None"
-    shows "ty_term (map_of (parameters (detype_ac a))) (ast_domain.constT detype_dom) x = Some \<omega>"
-    using assms detype_ac_def detype_dom_def t_tyt_some ast_domain.constT_def by auto
-
-  (* fun type_precond :: "(variable \<times> type) \<Rightarrow> term atom formula" where
-    "type_precond (v, T) =
-      disj_fmlas (map (Atom \<circ> (\<lambda>p. predAtm p [term.VAR v])) (type_conds T))"
-  
-  fun param_precond :: "(variable \<times> type) list \<Rightarrow> term atom formula" where
-    "param_precond params = conj_fmlas (map type_precond params)" *)
-
-  lemma conj_fmlas_wf:
+    lemma conj_fmlas_wf:
     assumes "\<forall>\<phi> \<in> set \<phi>s. wf_fmla tyt \<phi>"
     shows "wf_fmla tyt (conj_fmlas \<phi>s)"
     using assms apply (induction \<phi>s)
@@ -757,37 +662,65 @@ begin
     apply simp_all
     by (metis ast_domain.wf_fmla.simps(4) disj_fmlas.simps(2-3) neq_NilE)
 
-(* disj_fmlas (map (Atom \<circ> (\<lambda>p. predAtm p [term.VAR v])) (type_conds T)) *)
+text \<open> detype ac \<close>
 
-  lemma "\<forall>ent. snd (detype_ent ent) = \<omega>"
-    by simp
+  lemma ac_params_detyped:
+    "\<forall>ac \<in> set (actions D2). \<forall>(n, T) \<in> set (parameters ac). T = \<omega>"
+    using detype_dom_def detype_ac_def ents_detyped by fastforce
+
+  abbreviation "ac_name \<equiv> ast_action_schema.name"
+  (* abbreviation (in ast_domain) "ac_params \<equiv> ast_action_schema.parameters" \<comment> just use \<open>parameters\<close> *)
+  abbreviation "ac_pre \<equiv> ast_action_schema.precondition"
+  abbreviation "ac_eff \<equiv> ast_action_schema.effect"
+
+  lemma t_ac_name: "ac_name (detype_ac ac) = ac_name ac"
+    by (simp add: detype_ac_def)
+  lemma t_acs_names: "map ac_name (map detype_ac acs) = map ac_name acs"
+    by (simp add: t_ac_name)
+  lemma (in wf_ast_domain) t_acs_dis:
+    "distinct (map ac_name (map detype_ac (actions D)))"
+    using t_acs_names wf_dom_def by metis
+
+  (* TODO just manipulate lemma  *)
+  lemma wf_ac_expanded:
+    "wf_action_schema a \<longleftrightarrow> (
+      let
+        tyt = ty_term (map_of (parameters a)) constT
+      in
+        distinct (map fst (parameters a))
+      \<and> wf_fmla tyt (ac_pre a)
+      \<and> wf_effect tyt (ac_eff a))"
+    using wf_action_schema.simps
+    by (metis ast_action_schema.collapse)
+
+  lemma (in ast_domain2) t_ac_tyt:
+    assumes "ty_term (map_of (parameters a)) constT x \<noteq> None"
+    shows "ty_term (map_of (parameters (detype_ac a))) d2.constT x = Some \<omega>"
+    using assms detype_ac_def detype_dom_def t_tyt_Some ast_domain.constT_def by auto
 
   lemma params_ts_wf:
     assumes "wf_action_params a" "p \<in> set (parameters a)"
     shows "wf_type (snd p)"
     using assms wf_action_params_def by blast
 
-  lemma set_type_names: "set type_names = insert ''object'' (fst ` set (types D))" by auto
-
   lemma params_ts_exist: (* somehow this isn't trivial for the solver *)
     assumes "wf_action_params a" "p \<in> set (parameters a)"
     shows "\<forall>t \<in> set (primitives (snd p)). t \<in> insert ''object'' (set type_names)"
-    using assms params_ts_wf set_type_names
-    by (metis wf_type_iff_listed insertI2 type.exhaust_sel)
+    using assms params_ts_wf
+    by (metis wf_type_iff_listed insertI2)
 
-  lemma (in wf_ast_domain) type_precond_wf: (* TODO simplify if possible *)
+  lemma (in wf_ast_domain2) type_precond_wf: (* TODO simplify if possible *)
     assumes "wf_action_params a" "p \<in> set (parameters a)"
-    shows "ast_domain.wf_fmla detype_dom
-      (ty_term (map_of (parameters (detype_ac a))) egal)
+    shows "d2.wf_fmla
+      (ty_term (map_of (parameters (detype_ac a))) cnstT)
       (type_precond p)"
   proof -
-    interpret d2 : ast_domain detype_dom .
-    let ?tyt = "ty_term (map_of (parameters a)) egal"
-    let ?tyt2 = "ty_term (map_of (parameters (detype_ac a))) egal"
+    let ?tyt = "ty_term (map_of (parameters a)) cnstT"
+    let ?tyt2 = "ty_term (map_of (parameters (detype_ac a))) cnstT"
 
     have "?tyt (term.VAR (fst p)) \<noteq> None" using assms detype_ac_def
       by (metis imageI map_of_eq_None_iff ty_term.simps(1))
-    hence 1: "?tyt2 (term.VAR (fst p)) = Some \<omega>" using t_varT_some
+    hence 1: "?tyt2 (term.VAR (fst p)) = Some \<omega>" using t_tyt_var_Some
       by (simp add: detype_ac_def)
 
     have "\<forall>t \<in> set (primitives (snd p)). d2.wf_fmla ?tyt2 (Atom (predAtm (pred_for_type t) [term.VAR (fst p)]))"
@@ -795,8 +728,8 @@ begin
       fix t assume t: "t \<in> set (primitives (snd p))"
       have "t \<in> insert ''object'' (set type_names)" using assms params_ts_exist t by simp
       hence "PredDecl (pred_for_type t) [\<omega>] \<in> set type_preds" using type_preds_def by fastforce
-      moreover have "set type_preds \<subseteq> set (predicates detype_dom)" using detype_dom_def by simp
-      ultimately have "PredDecl (pred_for_type t) [\<omega>] \<in> set (predicates detype_dom)" by auto
+      moreover have "set type_preds \<subseteq> set (predicates D2)" using detype_dom_def by simp
+      ultimately have "PredDecl (pred_for_type t) [\<omega>] \<in> set (predicates D2)" by auto
       hence 2: "d2.sig (pred_for_type t) = Some [\<omega>]" using detype_dom_def
         by (metis d2.sig_def pred_resolve t_preds_dis) (* not true outside of restr_dom because action params need not wf *)
       from 1 2 show "d2.wf_fmla ?tyt2 (Atom (predAtm (pred_for_type t) [term.VAR (fst p)]))"
@@ -811,13 +744,12 @@ begin
       by (metis prod.collapse type_precond.simps)
   qed
 
-  lemma (in wf_ast_domain) t_param_precond_wf:
+  lemma (in wf_ast_domain2) t_param_precond_wf:
     assumes "wf_action_params a"
-    shows "ast_domain.wf_fmla detype_dom
+    shows "d2.wf_fmla
     (ty_term (map_of (parameters (detype_ac a))) egal)
     (param_precond (parameters a))"
   proof -
-    interpret d2 : ast_domain detype_dom .
     let ?tyt2 = "ty_term (map_of (parameters (detype_ac a))) egal"
     have "param_precond (parameters a) = conj_fmlas (map type_precond (parameters a))"
       by simp
@@ -830,11 +762,10 @@ begin
     thus ?thesis by simp
   qed
 
-  lemma (in restr_domain) t_ac_wf:
+  lemma (in restr_domain2) t_ac_wf:
     assumes "a \<in> set (actions D)"
-    shows "ast_domain.wf_action_schema detype_dom (detype_ac a)"
+    shows "d2.wf_action_schema (detype_ac a)"
   proof -
-    interpret d2 : ast_domain detype_dom .
     let ?a2 = "detype_ac a"
     let ?tyt = "ty_term (map_of (parameters a)) constT"
     let ?tyt2 = "ty_term (map_of (parameters (detype_ac a))) d2.constT"
@@ -857,15 +788,49 @@ begin
     from c1 c2 c3 show ?thesis using d2.wf_ac_expanded by simp
   qed
 
-  lemma (in restr_domain) t_acs_wf:
-    shows "(\<forall>a\<in>set (map detype_ac (actions D)). ast_domain.wf_action_schema detype_dom a)"
+  lemma (in restr_domain2) t_acs_wf:
+    shows "(\<forall>a\<in>set (map detype_ac (actions D)). d2.wf_action_schema a)"
     using detype_dom_def wf_dom_def t_ac_wf by simp
 
-  theorem (in restr_domain) detype_dom_wf:
-    shows "ast_domain.wf_domain detype_dom"
-  proof -
-    interpret d2 : ast_domain detype_dom .
+text \<open> init / goal \<close>
+
+lemma (in wf_ast_problem) t_init_dis: "distinct (init P2)"
+proof -
+  have "init P2 = supertype_facts (objects P) @ supertype_facts (consts D) @ (init P)"
+    using detype_prob_def by simp
+  show ?thesis sorry
+qed
   
+lemma (in wf_ast_problem2) t_init_wf:
+  "p2.wf_world_model (set (init P2))"
+  sorry
+
+
+text \<open> major\<close>
+  theorem (in ast_domain2) dom_detyped:
+    "d2.typeless_dom"
+  proof -
+    have c1: "types D2 = []" using detype_dom_def by simp
+    note c2 = preds_detyped
+    have c3: "\<forall>(n, T) \<in> set (consts D2). T = \<omega>"
+      by (simp add: detype_dom_def ents_detyped)
+    note c4 = ac_params_detyped
+  
+    from c1 c2 c3 c4 show ?thesis
+      using d2.typeless_dom_def by simp
+  qed
+
+  theorem (in ast_problem2) prob_detyped:
+    "p2.typeless_prob"
+  proof -
+    have "\<forall>(n, T) \<in> set (objects P2). T = \<omega>"
+      by (simp add: detype_prob_def ents_detyped)
+    thus ?thesis using dom_detyped p2.typeless_prob_def detype_prob_def by simp
+  qed
+
+  theorem (in restr_domain2) detype_dom_wf:
+    shows "d2.wf_domain"
+  proof -
     (* Types are well-formed because they are simply empty. *)
     have c1: "d2.wf_types" using d2.wf_types_def detype_dom_def by simp
     note c2 = t_preds_dis
@@ -882,61 +847,84 @@ begin
     from c1 c2 c3 c4 c5 c6 c7 show ?thesis
       using d2.wf_domain_def detype_dom_def by simp
   qed
+
+  theorem (in restr_problem2) detype_prob_wf:
+    shows "p2.wf_problem"
+  proof -
+    note c1 = detype_dom_wf
+    have "distinct (map fst (objects P) @ map fst (consts D))" using wf_prob_def by simp
+    hence c2: "distinct (map fst (detype_ents (objects P)) @ map fst (detype_ents (consts D)))"
+      using t_ents_names by metis
+    have c3: "\<forall>(n, y)\<in>set (objects P2). p2.wf_type y"
+      using t_ents_wf detype_prob_def by fastforce
+    note c4 = t_init_dis
+    note c5 = t_init_wf
+  
+    have c6a: "\<forall>e. objT e \<noteq> None \<longrightarrow> p2.objT e = Some \<omega>" using t_objT_Some by simp
+    have c6b: "wf_fmla objT (goal P2)" using detype_prob_def wf_prob_def by simp
+    have c6: "p2.wf_fmla p2.objT (goal P2)"
+      using t_fmla_wf[OF c6a c6b] detype_prob_def by simp
+    from c1 c2 c3 c4 c5 c6 show ?thesis
+      using p2.wf_problem_def detype_prob_def detype_dom_def by simp
+  qed
+
 end
 
-context ast_problem
+subsubsection \<open> Type Normalization Preserves Semantics \<close>
+
+context ast_domain
 begin
 
-lemmas (in wf_ast_problem) wf_prob_def = wf_problem[unfolded wf_problem_def]
+text \<open> Supertype Enumeration \<close>
 
-thm detype_prob_def
+  lemma of_type_iff_reach:
+    shows "of_type oT T \<longleftrightarrow> (
+      \<forall>ot \<in> set (primitives oT).
+      \<exists>t \<in> set (primitives T).
+        t \<in> set (supertypes_of ot))"
+  proof -
+    have "subtype_rel = set (map prod.swap (types D))"
+      using subtype_rel_def subtype_edge_swap by metis
+    hence subrel_inv: "subtype_rel = (set (types D))\<inverse>" by auto
+    hence "of_type oT T \<longleftrightarrow>
+      set (primitives oT) \<subseteq> ((set (types D))\<inverse>)\<^sup>* `` set (primitives T)"
+      using of_type_def by simp
+    also have "... \<longleftrightarrow>
+      set (primitives oT) \<subseteq> ((set (types D))\<^sup>*)\<inverse> `` set (primitives T)"
+      by (simp add: rtrancl_converse)
+    also have "... \<longleftrightarrow>
+      (\<forall>ot \<in> set (primitives oT). ot \<in> ((set (types D))\<^sup>*)\<inverse> `` set (primitives T))"
+      by auto
+    also have "... \<longleftrightarrow>
+      (\<forall>ot \<in> set (primitives oT). \<exists>t. (ot, t) \<in> (set (types D))\<^sup>* \<and> t \<in> set (primitives T))"
+      by auto
+    finally show ?thesis using reachable_iff_in_star by metis
+  qed
 
-lemma (in wf_ast_problem) t_init_dis: "distinct (init detype_prob)"
-  sorry
+  lemma (in ast_problem) obj_of_type_iff_reach:
+    assumes "objT n = Some oT"
+    shows  "is_obj_of_type n T \<longleftrightarrow>
+      (\<forall>ot \<in> set (primitives oT).
+        \<exists>t \<in> set (primitives T).
+      t \<in> set (supertypes_of ot))"
+    using assms is_obj_of_type_def of_type_iff_reach by auto
 
-thm wf_ast_domain.t_fmla_wf
+  lemma (in ast_domain) single_of_type_iff:
+    shows "of_type (Either [ot]) T \<longleftrightarrow> (
+      \<exists>t \<in> set (primitives T).
+        t \<in> set (supertypes_of ot))"
+    using of_type_iff_reach by simp
 
-theorem (in restr_problem) detype_prob_wf:
-  shows "ast_problem.wf_problem detype_prob"
-proof -
-  interpret p2 : ast_problem detype_prob .
+  lemma (in ast_problem) simple_obj_of_type_iff:
+    assumes "objT n = Some (Either [ot])"
+    shows  "is_obj_of_type n T \<longleftrightarrow>
+        (\<exists>t \<in> set (primitives T).
+      t \<in> set (supertypes_of ot))"
+    using assms is_obj_of_type_def single_of_type_iff by auto
 
-  note p2.wf_problem_def
-  note detype_prob_def
-
-  note c1 = detype_dom_wf
-  have "distinct (map fst (objects P) @ map fst (consts D))" using wf_prob_def by simp
-  hence c2: "distinct (map fst (detype_ents (objects P)) @ map fst (detype_ents (consts D)))"
-    using t_ents_names by metis
-  have c3: "\<forall>(n, y)\<in>set (objects detype_prob). p2.wf_type y" using t_ents_wf detype_prob_def by fastforce
-  note c4 = t_init_dis
-  have c5: "p2.wf_world_model (set (init detype_prob))" sorry
-
-  have c6a: "\<forall>e. objT e \<noteq> None \<longrightarrow> p2.objT e = Some \<omega>" sorry
-  have c6b: "wf_fmla objT (goal detype_prob)" using detype_prob_def wf_prob_def by simp
-  have c6: "p2.wf_fmla p2.objT (goal detype_prob)"
-    using t_fmla_wf[OF c6a c6b] detype_prob_def by simp
-  from c1 c2 c3 c4 c5 c6 show ?thesis
-    using p2.wf_problem_def detype_prob_def detype_dom_def by simp
-qed
 end
 
-
-(* ---------------------- Milestones ------------------------- *)
-
-
-(* TODO update locale hierarchy accordingly *)
-lemma (in restr_domain) "ast_domain.wf_domain detype_dom"
-  by (rule detype_dom_wf)
-
-lemma (in restr_problem) "ast_problem.wf_problem detype_prob"
-  by (rule detype_prob_wf)
-
-lemma "ast_domain.wf_domain D \<Longrightarrow> typeless_dom (detype_dom D)"
-  oops
-
-lemma "ast_problem.wf_problem P \<Longrightarrow> typeless_prob (detype_prob P)"
-  oops
+(* ---------------------- Future Milestones ------------------------- *)
 
 (* type normalization correct w.r.t. execution*)
 
