Utils.thy
@@ -26,6 +26,12 @@ fun conj_fmlas :: "'a formula list \<Rightarrow> 'a formula" where
 
 (* lemmas *)
 
+lemma map_of_SomeIn: "map_of m x = Some y \<Longrightarrow> y \<in> snd ` set m"
+  by (metis image_eqI map_of_SomeD snd_conv)
+
+lemma map_of_in_R_iff: "x \<in> fst ` set m \<longleftrightarrow> (\<exists>y. map_of m x = Some y \<and> y \<in> snd ` set m)"
+  using map_of_SomeIn
+  by (metis map_of_eq_None_iff not_None_eq)
 
 
 
